WIP: Added proof structure of ConcurSim

concur/MultiSim.v
@@ -12,7 +12,7 @@ Section ConcurSim.
 
   Variable OpenA : semantics li_asm li_asm.
 
-  Hypothesis OpenSim : forward_simulation cc_c_asm_injp cc_c_asm_injp OpenC OpenA.
+  (* Hypothesis OpenSim : forward_simulation cc_c_asm_injp cc_c_asm_injp OpenC OpenA. *)
 
   
   (** * Get the concurrent semantics *)
@@ -24,19 +24,102 @@ Section ConcurSim.
   Let se := CMulti.initial_se OpenC.
   Let tse := initial_se OpenA.
 
-  Definition main_id := prog_main (skel OpenA).
+  (*Definition main_id := prog_main (skel OpenA).
   
   Definition rs0 :=
     (Pregmap.init Vundef) # PC <- (Genv.symbol_address tse (main_id) Ptrofs.zero)
                           # RA <- Vnullptr
                           # RSP <- Vnullptr.
+   *)
+  Section FSIM.
 
-  
-  (** we cannot get the initial world if init_mem returns false, should we add it? *)
-  Let w0 := cajw (injpw ) main_sig rs0.
-  (** problem : do we need to change the index? *)
-  
-  Theorem ConcurSim : Closed.forward_simulation ConcurC ConcurA.
+    Variable fsim_index : Type.
+    Variable fsim_order : fsim_index -> fsim_index -> Prop.
+    Variable fsim_match_states : Genv.symtbl -> Genv.symtbl -> cc_cainjp_world -> fsim_index ->
+                                 Smallstep.state OpenC -> Smallstep.state OpenA -> Prop.
+    Hypothesis fsim_skel : skel OpenC = skel OpenA.
+    Hypothesis fsim_lts : forall (se1 se2 : Genv.symtbl) (wB : ccworld cc_c_asm_injp),
+        match_senv cc_c_asm_injp wB se1 se2 ->
+        Genv.valid_for (skel OpenC) se1 ->
+        fsim_properties cc_c_asm_injp cc_c_asm_injp se1 se2 wB (OpenC se1) 
+          (OpenA se2) fsim_index fsim_order (fsim_match_states se1 se2 wB).
+    
+    Hypothesis fsim_order_wf : well_founded fsim_order.
+    
+    (** Utilizing above properties *)
+    Definition match_local_states := fsim_match_states se tse.
+
+    Lemma MSE : se = tse.
+    Proof.
+      unfold se, tse. destruct OpenC, OpenA.
+      unfold CMulti.initial_se. unfold initial_se.
+      simpl in *. congruence.
+    Qed.
+
+    Lemma valid_se : Genv.valid_for (skel OpenC) se.
+    Proof.
+      unfold se. unfold CMulti.initial_se. red.
+      intros.
+      apply Genv.find_info_symbol in H. destruct H as [b [A B]].
+      exists b,g. split. auto. split. auto.
+      apply Linking.linkorder_refl.
+    Qed.
+    
+    (** Definition of match_state *)
+    Let thread_state_C := CMulti.thread_state OpenC.
+    Let thread_state_A := AsmMulti.thread_state OpenA.
+    
+    Inductive match_thread_states : cc_cainjp_world -> fsim_index -> thread_state_C -> thread_state_A -> Prop :=
+    |match_local : forall w i sc sa,
+        match_local_states w i sc sa ->
+        match_thread_states w i (CMulti.Local OpenC sc) (Local OpenA sa)
+    |match_initial : forall w i cqv rs m tm,
+        match_query cc_c_asm_injp w (get_query cqv m) (rs,tm) ->
+        match_thread_states w i (CMulti.Initial OpenC cqv) (Initial OpenA rs)
+    |match_return : forall w i sc sa qc rs tm,
+        match_local_states w i sc sa ->
+        (* match_query cc_c_asm_injp w ( )-> *)
+        query_is_yield OpenC qc ->
+        query_is_yield_asm OpenA (rs, tm) ->
+        match_query cc_c_asm_injp w qc (rs, tm) ->
+        match_thread_states w i (CMulti.Return OpenC sc) (Return OpenA sa rs).
+
+    (* Definition worlds : Type := NatMap.t (option cc_cainjp_world). *)
+    Definition empty_worlds : NatMap.t (option cc_cainjp_world) := NatMap.init None.
+    Definition initial_worlds (w: cc_cainjp_world) := NatMap.set 1%nat (Some w) empty_worlds.
+    
+    Inductive match_states : fsim_index -> CMulti.state OpenC -> state OpenA -> Prop :=
+    |global_match_intro : forall threadsC threadsA i cur next worlds
+      (THREADS: forall n, (1 <= n < next)%nat -> exists w lsc lsa i',
+            NatMap.get n worlds = Some w /\
+              NatMap.get n threadsC = Some lsc /\
+              NatMap.get n threadsA = Some lsa /\
+              match_thread_states w i' lsc lsa /\
+              fsim_order i' i),
+        match_states i (mk_gstate OpenC threadsC cur next) (mk_gstate_asm OpenA threadsA cur next).
+
+    Theorem Concur_Sim : Closed.forward_simulation ConcurC ConcurA.
+    Proof.
+      econstructor. instantiate (3:= fsim_index). instantiate (2:= fsim_order).
+      instantiate (1:= match_states).
+      constructor. auto.
+      - intros. inv H.
+        
+      Admitted.
+
+  End FSIM.
+
+  Lemma SIM : forward_simulation cc_c_asm_injp cc_c_asm_injp OpenC OpenA ->
+    Closed.forward_simulation ConcurC ConcurA.
   Proof.
-    inv OpenSim. inv X.
-    econstructor. 
+    intro. inv H. inv X. eapply Concur_Sim; eauto.
+  Qed.
+
+End ConcurSim.
+
+Theorem Opensim_to_Globalsim : forall OpenC OpenA,
+    forward_simulation cc_c_asm_injp cc_c_asm_injp OpenC OpenA ->
+    Closed.forward_simulation (Concur_sem_c OpenC) (Concur_sem_asm OpenA).
+Proof.
+  intros. eapply SIM; eauto.
+Qed.
